src/PrintHardwareEncoding.v
@@ -1,0 +1,60 @@
+From JSON Require Import Encode Printer.
+From Stdlib Require Import String List ZArith.
+From coqutil Require Import Map.Interface Result.
+From DatalogRocq Require Import EncodeLayout CompiledFamily.
+
+Instance JEncode__node_id : JEncode node_id :=
+  fun n => JSON__Object [("x", encode (fst n)); ("y", encode (snd n))].
+
+Instance JEncode__join : JEncode join :=
+  fun j =>
+    JSON__Object [("tries", encode j.(tries));
+                ("trie_levels", encode j.(trie_levels));
+                ("clauses", encode j.(clauses))].
+
+Instance JEncode__join_output : JEncode join_output := 
+  fun jo =>
+    JSON__Object [("output_rel", encode jo.(output_rel));
+                ("output_var_indices", encode jo.(output_var_indices))].
+
+Instance JEncode_hardware_rule : JEncode hardware_rule :=
+  fun hr =>
+    JSON__Object [("hhyps", encode hr.(hhyps));
+                ("hconcls", encode hr.(hconcls))].
+
+Instance JEncode__destination : JEncode destination := fun d =>
+  match d with
+  | DestEdge e => JSON__Object [("DestEdge", encode e)]
+  | DestTrie t => JSON__Object [("DestTrie", encode t)]
+  end.
+  
+
+Instance JEncode__pair A B `{JEncode A} `{JEncode B} : JEncode (A * B) :=
+  fun '(a, b) => JSON__Array [encode a; encode b].
+
+
+Instance JEncode_forwarding_table : JEncode (SortedListNat.map (list destination)) :=
+  fun m => encode (map.fold (fun acc k v => (k, v) :: acc) [] m).
+
+Instance JEncode__trie : JEncode trie :=
+  fun t =>
+    JSON__Object [("tid", encode t.(tid));
+                ("trel", encode t.(trel));
+                ("tperm", encode t.(tperm))].
+
+Instance JEncode__node_info : JEncode node_info :=
+  fun ni =>
+    JSON__Object [("nid", encode ni.(nid));
+                ("nprogram", encode ni.(nprogram));
+                ("nforwarding", encode ni.(nforwarding));
+                ("ntries", encode ni.(ntries))].
+
+
+Instance JEncode__Result {A} `{JEncode A} : JEncode (result A) :=
+  fun r =>
+  match r with
+  | Success a => encode a
+  | Failure _ => JSON__String "Failed to compile"
+  end.
+
+Redirect "json_examples/compiled_family_program" Eval vm_compute in (to_string (encode compiled_family)).
